Removed kind annotations in contexts

mechanization/theories/Core/Semantic/NbE.v
@@ -11,7 +11,7 @@ Inductive initial_env {P : PtsSig} : ctx P -> env P -> Prop :=
 | initial_env_cons :
   `( initial_env Γ ρ ->
      {{ ⟦ A ⟧ ρ ↘ a }} ->
-     initial_env ({{{ Γ, A::Sort@s }}}) d{{{ ρ ↦ ⇑! a (length Γ) }}}).
+     initial_env ({{{ Γ, A }}}) d{{{ ρ ↦ ⇑! a (length Γ) }}}).
 
 #[export]
 Hint Constructors initial_env : mcpts.
@@ -35,9 +35,9 @@ Hint Resolve functional_initial_env : mcpts.
     whether [a] is the evaluation result of A or not.
     If we want to specify that as well, we need a generalized
     version of [drop_env] that can drop [x] elements. *)
-Lemma initial_env_spec {P : PtsSig} : forall x (Γ : ctx P) ρ A s,
+Lemma initial_env_spec {P : PtsSig} : forall x (Γ : ctx P) ρ A,
     initial_env Γ ρ ->
-    {{ #x : A :: Sort@s ∈ Γ }} ->
+    {{ #x : A ∈ Γ }} ->
     exists m a, {{ ρ[x] ↘ m }} /\ m = d{{{ ⇑! a (length Γ - x - 1) }}}.
 Proof.
   induction x; intros * Hinit Hlookup;
