mechanization/theories/Core/Completeness/ContextCases.v
@@ -25,63 +25,63 @@ Qed.
 Hint Resolve rel_ctx_empty : mcpts.
 
 
-Lemma rel_ctx_extend {P : PtsSig} {pred_P : PredicativeSig P} : forall {Γ Γ' A A' s},
+(* Lemma rel_ctx_extend {P : PtsSig} {pred_P : PredicativeSig P} : forall {Γ Γ' A A'}, *)
+(*     {{ ⟪ pred_P ⟫ ⊨ Γ ≈ Γ' }} -> *)
+(*     {{ ⟪ pred_P ⟫ Γ ⊨ A ≈ A' }} -> *)
+(*     {{ ⟪ pred_P ⟫ ⊨ Γ, A ≈ Γ', A' }}. *)
+(* Proof with intuition. *)
+(*   intros * [] [env_relΓ]%rel_exp_of_typ_inversion1. *)
+(*   pose env_relΓ. *)
+(*   destruct_conjs. *)
+(*   handle_per_ctx_env_irrel. *)
+(*   eexists. *)
+(*   per_ctx_env_econstructor; eauto. *)
+(*   - instantiate (1 := fun ρ ρ' (equiv_ρ_ρ' : env_relΓ ρ ρ') m m' => *)
+(*                         forall s R, *)
+(*                           rel_typ pred_P s A ρ A' ρ' R -> *)
+(*                           R m m'). *)
+(*     intros. *)
+(*     (on_all_hyp: destruct_rel_by_assumption env_relΓ). *)
+(*     match_by_head (@per_sort P) ltac:(fun H => destruct H as [elem_relA]). *)
+(*     econstructor; eauto. *)
+(*     apply -> per_typ_elem_morphism_iff; eauto. *)
+(*     split; intros; destruct_by_head (@rel_typ P); handle_per_sort_elem_irrel... *)
+(*     assert (rel_typ pred_P s A ρ A' ρ' elem_relA) by mauto. *)
+(*     intuition. *)
+(*   - apply Equivalence_Reflexive. *)
+(* Qed. *)
+
+
+Lemma rel_ctx_extend {P : PtsSig} {pred_P : PredicativeSig P} : forall {Γ Γ' A A'},
     {{ ⟪ pred_P ⟫ ⊨ Γ ≈ Γ' }} ->
-    {{ ⟪ pred_P ⟫ Γ ⊨ A ≈ A' : Sort@s }} ->
-    {{ ⟪ pred_P ⟫ ⊨ Γ, A::Sort@s ≈ Γ', A'::Sort@s }}.
+    {{ ⟪ pred_P ⟫ Γ ⊨ A ≈ A' }} ->
+    {{ ⟪ pred_P ⟫ ⊨ Γ, A ≈ Γ', A' }}.
 Proof with intuition.
-  intros * [] [env_relΓ]%rel_exp_of_typ_inversion1.
+  intros * [] [env_relΓ]%rel_exp_of_typ_unsorted_inversion1.
   pose env_relΓ.
   destruct_conjs.
   handle_per_ctx_env_irrel.
   eexists.
   per_ctx_env_econstructor; eauto.
   - instantiate (1 := fun ρ ρ' (equiv_ρ_ρ' : env_relΓ ρ ρ') m m' =>
-                        forall s R,
-                          rel_typ pred_P s A ρ A' ρ' R ->
+                        forall R,
+                          rel_typ_unsorted pred_P A ρ A' ρ' R ->
                           R m m').
     intros.
     (on_all_hyp: destruct_rel_by_assumption env_relΓ).
-    match_by_head (@per_sort P) ltac:(fun H => destruct H as [elem_relA]).
+    match_by_head (@per_typ P) ltac:(fun H => destruct H as [elem_relA]).
     econstructor; eauto.
-    apply -> per_sort_elem_morphism_iff; eauto.
-    split; intros; destruct_by_head (@rel_typ P); handle_per_sort_elem_irrel...
-    assert (rel_typ pred_P s A ρ A' ρ' elem_relA) by mauto.
+    apply -> per_typ_elem_morphism_iff; eauto.
+    split; intros; destruct_by_head (@rel_typ_unsorted P); handle_per_typ_elem_irrel...
+    assert (rel_typ_unsorted pred_P A ρ A' ρ' elem_relA) by mauto.
     intuition.
   - apply Equivalence_Reflexive.
 Qed.
 
 
-Lemma rel_ctx_extend_unsorted {P : PtsSig} {pred_P : PredicativeSig P} : forall {Γ Γ' A A' s},
-    {{ ⟪ pred_P ⟫ ⊨ Γ ≈ Γ' }} ->
-    {{ ⟪ pred_P ⟫ Γ ⊨u A ≈ A' : Sort@s }} ->
-    {{ ⟪ pred_P ⟫ ⊨ Γ, A::Sort@s ≈ Γ', A'::Sort@s }}.
-Proof with intuition.
-  intros * [] [env_relΓ]%rel_exp_unsorted_of_typ_inversion1.
-  pose env_relΓ.
-  destruct_conjs.
-  handle_per_ctx_env_irrel.
-  eexists.
-  per_ctx_env_econstructor; eauto.
-  - instantiate (1 := fun ρ ρ' (equiv_ρ_ρ' : env_relΓ ρ ρ') m m' =>
-                        forall s R,
-                          rel_typ pred_P s A ρ A' ρ' R ->
-                          R m m').
-    intros.
-    (on_all_hyp: destruct_rel_by_assumption env_relΓ).
-    match_by_head (@per_sort P) ltac:(fun H => destruct H as [elem_relA]).
-    econstructor; eauto.
-    apply -> per_sort_elem_morphism_iff; eauto.
-    split; intros; destruct_by_head (@rel_typ P); handle_per_sort_elem_irrel...
-    assert (rel_typ pred_P s A ρ A' ρ' elem_relA) by mauto.
-    intuition.
-  - apply Equivalence_Reflexive.
-Qed.
-
-
-Lemma rel_ctx_extend' {P : PtsSig} {pred_P : PredicativeSig P} : forall {Γ A s},
-    {{ ⟪ pred_P ⟫ Γ ⊨ A : Sort@s }} ->
-    {{ ⟪ pred_P ⟫ ⊨ Γ, A::Sort@s }}.
+Lemma rel_ctx_extend' {P : PtsSig} {pred_P : PredicativeSig P} : forall {Γ A},
+    {{ ⟪ pred_P ⟫ Γ ⊨ A }} ->
+    {{ ⟪ pred_P ⟫ ⊨ Γ, A }}.
 Proof.
   intros.
   eapply rel_ctx_extend; eauto.
@@ -90,4 +90,4 @@ Proof.
 Qed.
 
 #[export]
-Hint Resolve rel_ctx_extend rel_ctx_extend_unsorted rel_ctx_extend' : mcpts.
+Hint Resolve rel_ctx_extend rel_ctx_extend' : mcpts.
