mechanization/theories/Core/Completeness/SubstitutionCases.v
@@ -16,9 +16,9 @@ Qed.
 #[export]
 Hint Resolve rel_sub_id : mcpts.
 
-Lemma rel_sub_weaken {P : PtsSig} {pred_P : PredicativeSig P} : forall {Γ A s},
-    {{ ⟪ pred_P ⟫ ⊨ Γ, A::Sort@s }} ->
-    {{ ⟪ pred_P ⟫ Γ, A::Sort@s ⊨s Wk ≈ Wk : Γ }}.
+Lemma rel_sub_weaken {P : PtsSig} {pred_P : PredicativeSig P} : forall {Γ A},
+    {{ ⟪ pred_P ⟫ ⊨ Γ, A }} ->
+    {{ ⟪ pred_P ⟫ Γ, A ⊨s Wk ≈ Wk : Γ }}.
 Proof with mautosolve.
   intros * [env_relΓA].
   invert_per_ctx_envs.
@@ -49,17 +49,17 @@ Qed.
 #[export]
 Hint Resolve rel_sub_compose_cong : mcpts.
 
-Lemma rel_sub_extend_cong {P : PtsSig} {pred_P : PredicativeSig P} : forall {s Γ M M' σ σ' Δ A},
+Lemma rel_sub_extend_cong {P : PtsSig} {pred_P : PredicativeSig P} : forall {Γ M M' σ σ' Δ A},
     {{ ⟪ pred_P ⟫ Γ ⊨s σ ≈ σ' : Δ }} ->
-    {{ ⟪ pred_P ⟫ Δ ⊨ A : Sort@s }} ->
-    {{ ⟪ pred_P ⟫ Γ ⊨ M ≈ M' : A[σ] }} ->
-    {{ ⟪ pred_P ⟫ Γ ⊨s σ ,, M ≈ σ' ,, M' : Δ, A::Sort@s }}.
+    {{ ⟪ pred_P ⟫ Δ ⊨ A }} ->
+    {{ ⟪ pred_P ⟫ Γ ⊨u M ≈ M' : A[σ] }} ->
+    {{ ⟪ pred_P ⟫ Γ ⊨s σ ,, M ≈ σ' ,, M' : Δ, A }}.
 Proof with mautosolve.
   intros * [env_relΓ [? [env_relΔ]]] HA [].
   destruct_conjs.
   pose env_relΓ.
   pose env_relΔ.
-  assert {{ ⟪ pred_P ⟫ ⊨ Δ, A::Sort@s }} as [] by (eapply rel_ctx_extend; eauto; eexists; mauto).
+  assert {{ ⟪ pred_P ⟫ ⊨ Δ, A }} as [] by (eapply rel_ctx_extend; eauto; eexists; mauto).
   handle_per_ctx_env_irrel.
   eexists_rel_sub.
   invert_per_ctx_envs.
@@ -67,54 +67,60 @@ Proof with mautosolve.
   intros.
   (on_all_hyp: destruct_rel_by_assumption env_relΓ).
   (on_all_hyp: destruct_rel_by_assumption env_relΔ).
-  destruct_by_head (@rel_typ P).
+  destruct_by_head (@rel_typ_unsorted P).
   invert_rel_typ_body.
   destruct_by_head (@rel_exp P).
-  econstructor; mauto;
-    econstructor; mauto;
-    econstructor; mauto.
+  econstructor; mauto.
+  econstructor; mauto; [econstructor; mauto | econstructor; mauto|].
+  assert (rel_typ_unsorted pred_P A ρ'0 A ρ'σ' (head_rel ρ'0 ρ'σ' H10)) by mauto.
+  destruct_by_head (@rel_typ_unsorted P).
+  simplify_evals.
+  assert (per_typ_elem pred_P elem_rel m m0) by mauto.
+  handle_per_typ_elem_irrel.
+  simpl.
+  eassumption.
 Qed.
 
 #[export]
 Hint Resolve rel_sub_extend_cong : mcpts.
 
 
-Lemma rel_sub_extend_cong_unsorted {P : PtsSig} {pred_P : PredicativeSig P} : forall {s Γ M M' σ σ' Δ A},
-    {{ ⟪ pred_P ⟫ Γ ⊨s σ ≈ σ' : Δ }} ->
-    {{ ⟪ pred_P ⟫ Δ ⊨u A : Sort@s }} ->
-    {{ ⟪ pred_P ⟫ Γ ⊨u M ≈ M' : A[σ] }} ->
-    {{ ⟪ pred_P ⟫ Γ ⊨s σ ,, M ≈ σ' ,, M' : Δ, A::Sort@s }}.
-Proof with mautosolve.
-  intros * [env_relΓ [? [env_relΔ]]] HA [].
-  destruct_conjs.
-  pose env_relΓ.
-  pose env_relΔ.
-  assert {{ ⟪ pred_P ⟫ ⊨ Δ, A::Sort@s }} as [] by (eapply rel_ctx_extend_unsorted; eauto; eexists; mauto).
-  handle_per_ctx_env_irrel.
-  eexists_rel_sub.
-  invert_per_ctx_envs_unsorted.
-  handle_per_ctx_env_irrel.
-  intros.
-  (on_all_hyp: destruct_rel_by_assumption env_relΓ).
-  (on_all_hyp: destruct_rel_by_assumption env_relΔ).
-  destruct_by_head (@rel_typ_unsorted P).
+(* Lemma rel_sub_extend_cong_unsorted {P : PtsSig} {pred_P : PredicativeSig P} : forall {s Γ M M' σ σ' Δ A}, *)
+(*     {{ ⟪ pred_P ⟫ Γ ⊨s σ ≈ σ' : Δ }} -> *)
+(*     {{ ⟪ pred_P ⟫ Δ ⊨ A }} -> *)
+(*     {{ ⟪ pred_P ⟫ Γ ⊨u M ≈ M' : A[σ] }} -> *)
+(*     {{ ⟪ pred_P ⟫ Γ ⊨s σ ,, M ≈ σ' ,, M' : Δ, A::Sort@s }}. *)
+(* Proof with mautosolve. *)
+(*   intros * [env_relΓ [? [env_relΔ]]] HA []. *)
+(*   destruct_conjs. *)
+(*   pose env_relΓ. *)
+(*   pose env_relΔ. *)
+(*   assert {{ ⟪ pred_P ⟫ ⊨ Δ, A::Sort@s }} as [] by (eapply rel_ctx_extend_unsorted; eauto; eexists; mauto). *)
+(*   handle_per_ctx_env_irrel. *)
+(*   eexists_rel_sub. *)
+(*   invert_per_ctx_envs_unsorted. *)
+(*   handle_per_ctx_env_irrel. *)
+(*   intros. *)
+(*   (on_all_hyp: destruct_rel_by_assumption env_relΓ). *)
+(*   (on_all_hyp: destruct_rel_by_assumption env_relΔ). *)
+(*   destruct_by_head (@rel_typ_unsorted P). *)
 
-  simplify_evals.
-  match_by_head (@per_typ_elem P) ltac:(fun H => directed inversion_clear H); subst.
-  clear_dups.
-  clear_refl_eqs.
-  handle_per_typ_elem_irrel.
-  clear_dups.
+(*   simplify_evals. *)
+(*   match_by_head (@per_typ_elem P) ltac:(fun H => directed inversion_clear H); subst. *)
+(*   clear_dups. *)
+(*   clear_refl_eqs. *)
+(*   handle_per_typ_elem_irrel. *)
+(*   clear_dups. *)
   
-  destruct_by_head (@rel_exp P).
-  econstructor; mauto.
-  econstructor; mauto;
-    econstructor; mauto;
-    econstructor; mauto.
-Qed.
+(*   destruct_by_head (@rel_exp P). *)
+(*   econstructor; mauto. *)
+(*   econstructor; mauto; *)
+(*     econstructor; mauto; *)
+(*     econstructor; mauto. *)
+(* Qed. *)
 
-#[export]
-Hint Resolve rel_sub_extend_cong_unsorted : mcpts.
+(* #[export] *)
+(* Hint Resolve rel_sub_extend_cong_unsorted : mcpts. *)
 
 
 Lemma rel_sub_id_compose_right {P : PtsSig} {pred_P : PredicativeSig P} : forall {Γ σ Δ},
@@ -167,19 +173,19 @@ Qed.
 #[export]
 Hint Resolve rel_sub_compose_assoc : mcpts.
 
-Lemma rel_sub_extend_compose {P : PtsSig} {pred_P : PredicativeSig P} : forall {Γ τ Γ' M σ Γ'' A s},
+Lemma rel_sub_extend_compose {P : PtsSig} {pred_P : PredicativeSig P} : forall {Γ τ Γ' M σ Γ'' A},
     {{ ⟪ pred_P ⟫ Γ' ⊨s σ : Γ'' }} ->
-    {{ ⟪ pred_P ⟫ Γ'' ⊨ A : Sort@s }} ->
-    {{ ⟪ pred_P ⟫ Γ' ⊨ M : A[σ] }} ->
+    {{ ⟪ pred_P ⟫ Γ'' ⊨ A }} ->
+    {{ ⟪ pred_P ⟫ Γ' ⊨u M : A[σ] }} ->
     {{ ⟪ pred_P ⟫ Γ ⊨s τ : Γ' }} ->
-    {{ ⟪ pred_P ⟫ Γ ⊨s (σ ,, M) ∘ τ ≈ (σ ∘ τ) ,, M[τ] : Γ'', A::Sort@s }}.
+    {{ ⟪ pred_P ⟫ Γ ⊨s (σ ,, M) ∘ τ ≈ (σ ∘ τ) ,, M[τ] : Γ'', A }}.
 Proof with mautosolve.
   intros * [env_relΓ' [? [env_relΓ'']]] HA [] [env_relΓ].
   destruct_conjs.
   pose env_relΓ'.
   pose env_relΓ''.
   handle_per_ctx_env_irrel.
-  assert {{ ⟪ pred_P ⟫ ⊨ Γ'', A::Sort@s }} as [] by (eapply rel_ctx_extend_unsorted; mauto; econstructor; mauto).
+  assert {{ ⟪ pred_P ⟫ ⊨ Γ'', A }} as [] by (eapply rel_ctx_extend; mauto; econstructor; mauto).
   destruct_conjs.
   eexists_rel_sub.
   invert_per_ctx_envs_unsorted.
@@ -190,7 +196,6 @@ Proof with mautosolve.
   (on_all_hyp: destruct_rel_by_assumption env_relΓ'').
   assert (rel_typ_unsorted pred_P {{{ A[σ] }}} ρσ {{{ A[σ] }}} ρ'σ' elem_rel) by mauto.
   destruct_by_head (@rel_typ_unsorted P).
-  destruct_by_head (@rel_typ P).
   
   simplify_evals.
   match_by_head (@per_typ_elem P) ltac:(fun H => directed inversion_clear H); subst.
@@ -212,75 +217,75 @@ Hint Resolve rel_sub_extend_compose : mcpts.
 
 
 
-Lemma rel_sub_extend_compose_unsorted {P : PtsSig} {pred_P : PredicativeSig P} : forall {Γ τ Γ' M σ Γ'' A s},
-    {{ ⟪ pred_P ⟫ Γ' ⊨s σ : Γ'' }} ->
-    {{ ⟪ pred_P ⟫ Γ'' ⊨u A : Sort@s }} ->
-    {{ ⟪ pred_P ⟫ Γ' ⊨u M : A[σ] }} ->
-    {{ ⟪ pred_P ⟫ Γ ⊨s τ : Γ' }} ->
-    {{ ⟪ pred_P ⟫ Γ ⊨s (σ ,, M) ∘ τ ≈ (σ ∘ τ) ,, M[τ] : Γ'', A::Sort@s }}.
-Proof with mautosolve.
-  intros * [env_relΓ' [? [env_relΓ'']]] HA [] [env_relΓ].
-  destruct_conjs.
-  pose env_relΓ'.
-  pose env_relΓ''.
-  handle_per_ctx_env_irrel.
-  assert {{ ⟪ pred_P ⟫ ⊨ Γ'', A::Sort@s }} as [] by (eapply rel_ctx_extend_unsorted; eauto; eexists; eassumption).
-  destruct_conjs.
-  eexists_rel_sub.
-  invert_per_ctx_envs_unsorted.
-  handle_per_ctx_env_irrel.
-  intros.
-  (on_all_hyp: destruct_rel_by_assumption env_relΓ).
-  (on_all_hyp: destruct_rel_by_assumption env_relΓ').
-  (on_all_hyp: destruct_rel_by_assumption env_relΓ'').
-  assert (rel_typ_unsorted pred_P A ρσ0 A ρ'σ'0 (head_rel ρσ0 ρ'σ'0 H13)) by mauto.
-  destruct_by_head (@rel_typ_unsorted P).
+(* Lemma rel_sub_extend_compose_unsorted {P : PtsSig} {pred_P : PredicativeSig P} : forall {Γ τ Γ' M σ Γ'' A s}, *)
+(*     {{ ⟪ pred_P ⟫ Γ' ⊨s σ : Γ'' }} -> *)
+(*     {{ ⟪ pred_P ⟫ Γ'' ⊨u A : Sort@s }} -> *)
+(*     {{ ⟪ pred_P ⟫ Γ' ⊨u M : A[σ] }} -> *)
+(*     {{ ⟪ pred_P ⟫ Γ ⊨s τ : Γ' }} -> *)
+(*     {{ ⟪ pred_P ⟫ Γ ⊨s (σ ,, M) ∘ τ ≈ (σ ∘ τ) ,, M[τ] : Γ'', A::Sort@s }}. *)
+(* Proof with mautosolve. *)
+(*   intros * [env_relΓ' [? [env_relΓ'']]] HA [] [env_relΓ]. *)
+(*   destruct_conjs. *)
+(*   pose env_relΓ'. *)
+(*   pose env_relΓ''. *)
+(*   handle_per_ctx_env_irrel. *)
+(*   assert {{ ⟪ pred_P ⟫ ⊨ Γ'', A::Sort@s }} as [] by (eapply rel_ctx_extend_unsorted; eauto; eexists; eassumption). *)
+(*   destruct_conjs. *)
+(*   eexists_rel_sub. *)
+(*   invert_per_ctx_envs_unsorted. *)
+(*   handle_per_ctx_env_irrel. *)
+(*   intros. *)
+(*   (on_all_hyp: destruct_rel_by_assumption env_relΓ). *)
+(*   (on_all_hyp: destruct_rel_by_assumption env_relΓ'). *)
+(*   (on_all_hyp: destruct_rel_by_assumption env_relΓ''). *)
+(*   assert (rel_typ_unsorted pred_P A ρσ0 A ρ'σ'0 (head_rel ρσ0 ρ'σ'0 H13)) by mauto. *)
+(*   destruct_by_head (@rel_typ_unsorted P). *)
 
-  simplify_evals.
-  match_by_head (@per_typ_elem P) ltac:(fun H => directed inversion_clear H); subst.
-  clear_dups.
-  clear_refl_eqs.
-  handle_per_typ_elem_irrel.
-  clear_dups.
+(*   simplify_evals. *)
+(*   match_by_head (@per_typ_elem P) ltac:(fun H => directed inversion_clear H); subst. *)
+(*   clear_dups. *)
+(*   clear_refl_eqs. *)
+(*   handle_per_typ_elem_irrel. *)
+(*   clear_dups. *)
   
-  destruct_by_head (@rel_exp P).
-  econstructor; mauto.
+(*   destruct_by_head (@rel_exp P). *)
+(*   econstructor; mauto. *)
 
-  econstructor; mauto;
-    econstructor; mauto;
-    econstructor; mauto.
-Qed.
+(*   econstructor; mauto; *)
+(*     econstructor; mauto; *)
+(*     econstructor; mauto. *)
+(* Qed. *)
 
-#[export]
-Hint Resolve rel_sub_extend_compose_unsorted : mcpts.
+(* #[export] *)
+(* Hint Resolve rel_sub_extend_compose_unsorted : mcpts. *)
+
+
+
+(* Lemma rel_sub_p_extend {P : PtsSig} {pred_P : PredicativeSig P} : forall {Γ' M σ Γ A}, *)
+(*     {{ ⟪ pred_P ⟫ Γ' ⊨s σ : Γ }} -> *)
+(*     {{ ⟪ pred_P ⟫ Γ' ⊨ M : A[σ] }} -> *)
+(*     {{ ⟪ pred_P ⟫ Γ' ⊨s Wk ∘ (σ ,, M) ≈ σ : Γ }}. *)
+(* Proof with mautosolve. *)
+(*   intros * [env_relΓ'] []. *)
+(*   destruct_conjs. *)
+(*   pose env_relΓ'. *)
+(*   handle_per_ctx_env_irrel. *)
+(*   eexists_rel_sub. *)
+(*   intros. *)
+(*   (on_all_hyp: destruct_rel_by_assumption env_relΓ'). *)
+(*   destruct_by_head (@rel_typ P). *)
+(*   invert_rel_typ_body. *)
+(*   destruct_by_head (@rel_exp P). *)
+(*   econstructor... *)
+(* Qed. *)
+
+(* #[export] *)
+(* Hint Resolve rel_sub_p_extend : mcpts. *)
+
 
 
 
 Lemma rel_sub_p_extend {P : PtsSig} {pred_P : PredicativeSig P} : forall {Γ' M σ Γ A},
-    {{ ⟪ pred_P ⟫ Γ' ⊨s σ : Γ }} ->
-    {{ ⟪ pred_P ⟫ Γ' ⊨ M : A[σ] }} ->
-    {{ ⟪ pred_P ⟫ Γ' ⊨s Wk ∘ (σ ,, M) ≈ σ : Γ }}.
-Proof with mautosolve.
-  intros * [env_relΓ'] [].
-  destruct_conjs.
-  pose env_relΓ'.
-  handle_per_ctx_env_irrel.
-  eexists_rel_sub.
-  intros.
-  (on_all_hyp: destruct_rel_by_assumption env_relΓ').
-  destruct_by_head (@rel_typ P).
-  invert_rel_typ_body.
-  destruct_by_head (@rel_exp P).
-  econstructor...
-Qed.
-
-#[export]
-Hint Resolve rel_sub_p_extend : mcpts.
-
-
-
-
-Lemma rel_sub_p_extend_unsorted {P : PtsSig} {pred_P : PredicativeSig P} : forall {Γ' M σ Γ A},
     {{ ⟪ pred_P ⟫ Γ' ⊨s σ : Γ }} ->
     {{ ⟪ pred_P ⟫ Γ' ⊨u M : A[σ] }} ->
     {{ ⟪ pred_P ⟫ Γ' ⊨s Wk ∘ (σ ,, M) ≈ σ : Γ }}.
@@ -306,13 +311,13 @@ Proof with mautosolve.
 Qed.
 
 #[export]
-Hint Resolve rel_sub_p_extend_unsorted : mcpts.
+Hint Resolve rel_sub_p_extend : mcpts.
 
 
 
-Lemma rel_sub_extend {P : PtsSig} {pred_P : PredicativeSig P} : forall {Γ' σ Γ A s},
-    {{ ⟪ pred_P ⟫ Γ' ⊨s σ : Γ, A::Sort@s }} ->
-    {{ ⟪ pred_P ⟫ Γ' ⊨s σ ≈ (Wk ∘ σ) ,, #0[σ] : Γ, A::Sort@s }}.
+Lemma rel_sub_extend {P : PtsSig} {pred_P : PredicativeSig P} : forall {Γ' σ Γ A},
+    {{ ⟪ pred_P ⟫ Γ' ⊨s σ : Γ, A }} ->
+    {{ ⟪ pred_P ⟫ Γ' ⊨s σ ≈ (Wk ∘ σ) ,, #0[σ] : Γ, A }}.
 Proof with mautosolve.
   intros * [env_relΓ' [? [env_relΓA]]].
   destruct_conjs.
@@ -325,9 +330,7 @@ Proof with mautosolve.
   (on_all_hyp: destruct_rel_by_assumption env_relΓ').
   inversion_by_head (@cons_per_ctx_env P); subst.
   (on_all_hyp: destruct_rel_by_assumption env_relΓ).
-  econstructor; mauto.
-  econstructor; mauto.
-  econstructor; mauto.
+  do 3 (econstructor; mauto).
 Qed.
 
 #[export]
