mechanization/theories/Core/Semantic/PER/Definitions.v
@@ -346,9 +346,9 @@ Section Per_ctx_env_def.
           (equiv_Γ_Γ' : {{ EF Γ ≈ Γ' ∈ per_ctx_env ↘ tail_rel }}),
           PER tail_rel ->
           (forall {ρ ρ'} (equiv_ρ_ρ' : {{ Dom ρ ≈ ρ' ∈ tail_rel }}),
-              rel_typ pred_P s A ρ A' ρ' (head_rel equiv_ρ_ρ')) ->
+              rel_typ_unsorted pred_P A ρ A' ρ' (head_rel equiv_ρ_ρ')) ->
           (env_rel <~> cons_per_ctx_env tail_rel (@head_rel)) ->
-          {{ EF Γ, A::Sort@s ≈ Γ', A'::Sort@s ∈ per_ctx_env ↘ env_rel }} }
+          {{ EF Γ, A ≈ Γ', A' ∈ per_ctx_env ↘ env_rel }} }
   .
 End Per_ctx_env_def.
 
