mechanization/theories/Core/Syntactic/Corollaries.v
@@ -37,9 +37,9 @@ Proof.
   intros * H.
   inversion_clear H.
   - assert {{ Γ ⊢ A : Sort@s }} by mauto.
-    mauto.
+    mauto 2.
   - assert {{ ⊢ Γ ≈ Δ }} by mauto.
-    mauto.
+    mauto 3.
 Qed.
 
 Hint Resolve invert_typ_id : mcpts.
@@ -88,50 +88,46 @@ Proof. induction 1; simpl; auto. Qed.
 
 Open Scope list_scope.
 
-Lemma app_ctx_lookup {P : PtsSig} : forall (Δ : ctx P) T Γ n K,
+Lemma app_ctx_lookup {P : PtsSig} : forall (Δ : ctx P) T Γ n,
     length Δ = n ->
-    {{ #n : ^(iter (S n) (fun T => {{{ T[Wk] }}}) T) :: K ∈ ^(Δ ++ (T, K) :: Γ) }}.
+    {{ #n : ^(iter (S n) (fun T => {{{ T[Wk] }}}) T) ∈ ^(Δ ++ T :: Γ) }}.
 Proof.
   induction Δ; intros; simpl in *; subst; mauto.
-  assert {{ # (length Δ) : ^ (iter (length Δ) (fun T0 => {{{ T0[Wk] }}}) T)[Wk] :: K ∈ ^ (app Δ {{{ Γ, T::K }}}) }} by mauto.
-  destruct_conjs.
-  mauto.
 Qed.  
 
-Lemma ctx_lookup_functional {P : PtsSig} : forall n (T : exp P) K Γ,
-    {{ #n : T :: K ∈ Γ }} ->
-    forall T' K',
-      {{ #n : T' :: K' ∈ Γ }} ->
-      T = T' /\ K = K'.
+Lemma ctx_lookup_functional {P : PtsSig} : forall n (T : exp P) Γ,
+    {{ #n : T ∈ Γ }} ->
+    forall T',
+      {{ #n : T' ∈ Γ }} ->
+      T = T'.
 Proof.
   induction 1; intros; progressive_inversion; eauto.
-  assert ((A = A0) /\ (K = K')) by mauto.
-  destruct_conjs; subst.
+  assert (A = A0) by mauto.
+  subst.
   mauto.
 Qed.
 
-Lemma app_ctx_vlookup {P : PtsSig} : forall (Δ : ctx P) T Γ n K,
-    {{ ⊢ ^(Δ ++ (T, K) :: Γ) }} ->
+Lemma app_ctx_vlookup {P : PtsSig} : forall (Δ : ctx P) T Γ n,
+    {{ ⊢ ^(Δ ++ T :: Γ) }} ->
     length Δ = n ->
-    {{ ^(Δ ++ (T, K) :: Γ) ⊢ #n : ^(iter (S n) (fun T => {{{ T[Wk] }}}) T) }}.
+    {{ ^(Δ ++ T :: Γ) ⊢ #n : ^(iter (S n) (fun T => {{{ T[Wk] }}}) T) }}.
 Proof.
   intros.
-  assert {{ #n : ^(iter (S n) (fun T' => {{{ T'[Wk] }}}) T) :: K ∈ ^(Δ ++ (T, K) :: Γ) }} by (eapply app_ctx_lookup; mauto).
-  assert (exists s, K = {{{ Sort@s }}}) by (eapply presup_ctx_lookup_typ; mauto).
-  destruct_conjs; subst.
+  assert {{ #n : ^(iter (S n) (fun T' => {{{ T'[Wk] }}}) T) ∈ ^(Δ ++ T :: Γ) }} by (eapply app_ctx_lookup; mauto).
+  subst.
   econstructor; mauto.
 Qed.
 
-Lemma sub_q_eq {P : PtsSig} : forall (Δ : ctx P) A s Γ σ σ',
-    {{ Δ ⊢ A : Sort@s }} ->
+Lemma sub_q_eq {P : PtsSig} : forall (Δ : ctx P) A Γ σ σ',
+    {{ Δ ⊢ A }} ->
     {{ Γ ⊢s σ ≈ σ' : Δ }} ->
-    {{ Γ, A[σ]::Sort@s ⊢s q σ ≈ q σ' : Δ, A::Sort@s }}.
+    {{ Γ, A[σ] ⊢s q σ ≈ q σ' : Δ, A }}.
 Proof.
   intros. gen_presup H0.
   econstructor; mauto 3.
   - econstructor; mauto 4.
-  - assert {{ #0 : A[σ][Wk] :: Sort@s ∈ Γ, A[σ]::Sort@s }} by mauto.
-    assert {{ Γ, A[σ]::Sort@s ⊢ #0 ≈ #0 : A[σ][Wk] }} by mauto.
+  - assert {{ #0 : A[σ][Wk] ∈ Γ, A[σ] }} by mauto.
+    assert {{ Γ, A[σ] ⊢ #0 ≈ #0 : A[σ][Wk] }} by mauto.
     eapply wf_exp_eq_conv'; mauto.
 Qed.
 #[export]
@@ -167,29 +163,33 @@ Qed.
 #[export]
 Hint Resolve exp_typ_sub_lhs : mcpts.
 
-Lemma sub_decompose_q {P : PtsSig} : forall (Γ : ctx P) A s σ Δ Δ' τ M,
-  {{ Γ ⊢ A : Sort@s }} ->
+Lemma sub_decompose_q {P : PtsSig} : forall (Γ : ctx P) A σ Δ Δ' τ M,
+  {{ Γ ⊢ A }} ->
   {{ Δ ⊢s σ : Γ }} ->
   {{ Δ' ⊢s τ : Δ }} ->
   {{ Δ' ⊢ M : A[σ][τ] }} ->
-  {{ Δ' ⊢s q σ ∘ (τ ,, M) ≈ σ ∘ τ ,, M : Γ, A::Sort@s }}.
+  {{ Δ' ⊢s q σ ∘ (τ ,, M) ≈ σ ∘ τ ,, M : Γ, A }}.
 Proof.
   intros. gen_presups.
   simpl.
   rewrite wf_sub_eq_extend_compose; mauto 3.
-  - assert {{ Δ' ⊢s (σ∘Wk)∘(τ,,M) ≈ σ∘(Wk∘(τ,,M)) : Γ }} by (eapply wf_sub_eq_compose_assoc; mauto).
+  - assert {{ Δ' ⊢s (σ∘Wk)∘(τ,,M) ≈ σ∘(Wk∘(τ,,M)) : Γ }}.
+    {
+      eapply wf_sub_eq_compose_assoc; mauto 3.
+      econstructor; mauto 3.
+    }
     assert {{ Δ' ⊢s σ∘(Wk∘(τ,,M)) ≈ σ∘τ : Γ }} by (eapply wf_sub_eq_compose_cong; mauto).
     assert {{ Δ' ⊢s (σ∘Wk)∘(τ,,M) ≈ σ∘τ : Γ}} by (etransitivity; mauto).
     assert {{ Δ' ⊢ #0[τ,,M] ≈ M : A[σ][τ] }} by (eapply wf_exp_eq_var_0_sub; mauto).
-    eapply wf_sub_eq_extend_cong; mauto.
+    eapply wf_sub_eq_extend_cong; mauto 2.
     assert {{ Γ ⊢ A ≈ A }} by mauto.
     assert {{ Δ' ⊢ A[σ][τ] ≈ A[σ∘τ] }} by mauto.
     assert {{ Δ' ⊢ A[σ∘τ] ≈ A[(σ∘Wk)∘(τ,,M)] }} by mauto.
     assert {{ Δ' ⊢ A[σ][τ] ≈ A[(σ∘Wk)∘(τ,,M)] }} by (etransitivity; mauto).
-    eapply wf_exp_eq_conv; mauto.
-  - mauto.
-  - assert {{ Δ, A[σ]::Sort@s ⊢ A[σ][Wk] ≈ A[σ∘Wk] }} by (eapply exp_eq_sub_compose_typ; mauto).
-    assert {{ #0 : A[σ][Wk] :: Sort@s ∈ Δ, A[σ]::Sort@s }} by mauto.
+    eapply wf_exp_eq_conv; mauto 4.
+  - mauto 5.
+  - assert {{ Δ, A[σ] ⊢ A[σ][Wk] ≈ A[σ∘Wk] }} by (eapply exp_eq_sub_compose_typ; mauto 4).
+    assert {{ #0 : A[σ][Wk] ∈ Δ, A[σ] }} by mauto.
     gen_presup H3.
     eapply wf_exp_conv with (A := {{{ A[σ][Wk] }}}); mauto.
 Qed.
@@ -197,42 +197,37 @@ Qed.
 #[local]
 Hint Rewrite -> @sub_decompose_q using mauto : mcpts.
 
-Lemma sub_decompose_q_typ {P : PtsSig} : forall (Γ : ctx P) A B s1 s2 σ Δ Δ' τ M,
-  {{ Γ, A::Sort@s1 ⊢ B : Sort@s2 }} ->
+Lemma sub_decompose_q_typ {P : PtsSig} : forall (Γ : ctx P) A B σ Δ Δ' τ M,
+  {{ Γ, A ⊢ B }} ->
   {{ Δ ⊢s σ : Γ }} ->
   {{ Δ' ⊢s τ : Δ }} ->
   {{ Δ' ⊢ M : A[σ][τ] }} ->
-  {{ Δ' ⊢ B[σ∘τ,,M] ≈ B[q σ][τ,,M] : Sort@s2 }}.
+  {{ Δ' ⊢ B[σ∘τ,,M] ≈ B[q σ][τ,,M] }}.
 Proof.
   intros. gen_presups.
-  assert {{ Δ' ⊢s q σ ∘ (τ ,, M) ≈ σ ∘ τ ,, M : Γ, A::Sort@s1 }} by (eapply sub_decompose_q; mauto 2).
+  assert {{ Δ' ⊢s q σ ∘ (τ ,, M) ≈ σ ∘ τ ,, M : Γ, A }} by (eapply sub_decompose_q; mauto 2).
   transitivity {{{ B[(q σ)∘(τ,,M)] }}}.
-  - eapply wf_exp_eq_conv' with (A := {{{ Sort@s2[σ∘τ,,M] }}}).
-    eapply wf_exp_eq_sub_cong; mauto 2.
-    do 2 (econstructor; mauto 2); eapply wf_conv'; mauto.
-  - eapply wf_exp_eq_conv' with (A := {{{ Sort@s2[(q σ)∘(τ,,M)] }}}).
-    eapply wf_exp_eq_sub_compose; mauto.
-    econstructor; mauto 3.
-    gen_presup H3.
-    mauto 2.
+  - eapply wf_typ_eq_sub_cong; mauto 2.
+  - eapply wf_typ_eq_sub_compose; mauto 4.
 Qed.
 
-Lemma sub_eq_p_q_sigma_compose_tau_extend {P : PtsSig} : forall {Δ' : ctx P} {τ Δ M A s σ Γ},
+Lemma sub_eq_p_q_sigma_compose_tau_extend {P : PtsSig} : forall {Δ' : ctx P} {τ Δ M A σ Γ},
     {{ Δ ⊢s σ : Γ }} ->
     {{ Δ' ⊢s τ : Δ }} ->
-    {{ Γ ⊢ A : Sort@s }} ->
+    {{ Γ ⊢ A }} ->
     {{ Δ' ⊢ M : A[σ][τ] }} ->
     {{ Δ' ⊢s Wk∘(q σ∘(τ,,M)) ≈ σ∘τ : Γ }}.
 Proof.
   intros.
-  assert {{ ⊢ Γ, A::Sort@s }} by mauto 3.
-  assert {{ Δ, A[σ]::Sort@s ⊢s q σ : Γ, A::Sort@s }} by mauto 2.
-  assert {{ Δ' ⊢s τ,,M : Δ, A[σ]::Sort@s }} by mauto 3.
+  assert {{ ⊢ Γ, A }} by mauto 3.
+  assert {{ Δ, A[σ] ⊢s q σ : Γ, A }} by mauto 2.
+  assert {{ Δ' ⊢s τ,,M : Δ, A[σ] }} by mauto 3.
   transitivity {{{ Wk∘((σ∘τ),,M) }}}; [| autorewrite with mcpts; mauto 3].
   eapply wf_sub_eq_compose_cong; [| mauto 2].
-  autorewrite with mcpts. econstructor; mauto 3.
-  assert {{ Δ' ⊢ A[σ∘τ] ≈ A[σ][τ] : Sort@s }} as -> by mauto.
-  mauto 3.
+  autorewrite with mcpts.
+  econstructor; mauto 3.
+  assert {{ Δ' ⊢ A[σ∘τ] ≈ A[σ][τ] }} by mauto.
+  eapply wf_exp_eq_conv; mauto 3.
 Qed.
 
 #[export]
@@ -242,56 +237,54 @@ Hint Rewrite -> @sub_eq_p_q_sigma_compose_tau_extend using mauto 4 : mcpts.
 
 
 (** This works for both natrec_sub and app_sub cases *)
-Lemma exp_eq_elim_sub_lhs_typ_gen {P : PtsSig} : forall {Γ : ctx P} {σ Δ M A B s1 s2},
+Lemma exp_eq_elim_sub_lhs_typ_gen {P : PtsSig} : forall {Γ : ctx P} {σ Δ M A B},
     {{ Γ ⊢s σ : Δ }} ->
-    {{ Δ, A::Sort@s1 ⊢ B : Sort@s2 }} ->
+    {{ Δ, A ⊢ B }} ->
     {{ Δ ⊢ M : A }} ->
-    {{ Γ ⊢ B[Id,,M][σ] ≈ B[σ,,M[σ]] : Sort@s2 }}.
+    {{ Γ ⊢ B[Id,,M][σ] ≈ B[σ,,M[σ]] }}.
 Proof.
   intros.
   assert {{ ⊢ Δ }} by mauto 2.
-  assert ({{ Δ ⊢ A : Sort@s1 }}) by mauto 3.
-  assert {{ Δ ⊢s Id,,M : Δ, A::Sort@s1 }} by mauto 4.
+  assert ({{ Δ ⊢ A }}) by mauto 3.
+  assert {{ Δ ⊢s Id,,M : Δ, A }} by mauto 4.
   autorewrite with mcpts.
   assert {{ Γ ⊢ M[σ] : A[σ] }} by mauto 2.
-  assert {{ Γ ⊢s σ,,M[σ] ≈ (Id,,M)∘σ : Δ, A::Sort@s1 }} as -> by mauto.
-  eapply wf_exp_eq_conv'; mauto 4.
+  assert {{ Γ ⊢s σ,,M[σ] ≈ (Id,,M)∘σ : Δ, A }} by mauto.
+  eapply wf_typ_eq_sub_cong; mauto 2.
 Qed.
 #[export]
 Hint Resolve exp_eq_elim_sub_lhs_typ_gen : mcpts.
 
 (** This works for both natrec_sub and app_sub cases *)
-Lemma exp_eq_elim_sub_rhs_typ {P : PtsSig} : forall {Γ : ctx P} {σ Δ M A B s1 s2},
+Lemma exp_eq_elim_sub_rhs_typ {P : PtsSig} : forall {Γ : ctx P} {σ Δ M A B},
     {{ Γ ⊢s σ : Δ }} ->
-    {{ Δ, A::Sort@s1 ⊢ B : Sort@s2 }} ->
+    {{ Δ, A ⊢ B }} ->
     {{ Γ ⊢ M : A[σ] }} ->
-    {{ Γ ⊢ B[q σ][Id,,M] ≈ B[σ,,M] : Sort@s2 }}.
+    {{ Γ ⊢ B[q σ][Id,,M] ≈ B[σ,,M] }}.
 Proof.
   intros.
-  assert ({{ Δ ⊢ A : Sort@s1 }}) by mauto 3.
+  assert ({{ Δ ⊢ A }}) by mauto 3.
   transitivity {{{ B[(σ∘Id),,M] }}}.
-  symmetry.
-  eapply sub_decompose_q_typ; mauto.
-  assert {{ Γ ⊢s σ∘Id,,M ≈ σ,,M : Δ, A::Sort@s1 }}.
-  {
+  - symmetry.
+    eapply sub_decompose_q_typ; mauto 2.
+    assert {{ Γ ⊢s σ∘Id,,M ≈ σ,,M : Δ, A }}.
+    {
+      eapply wf_sub_eq_extend_cong; mauto 2.
+      eapply wf_exp_eq_conv'; mauto.
+    }
+    econstructor; mauto 2.
+  - eapply wf_typ_eq_sub_cong; mauto 2.
     eapply wf_sub_eq_extend_cong; mauto 2.
     eapply wf_exp_eq_conv'; mauto.
-  }
-  eapply wf_exp_eq_conv'; mauto.
-  do 2 (econstructor; mauto 2).
-  econstructor; mauto.
-  eapply wf_conv'; mauto.
 Qed.
 #[export]
 Hint Resolve exp_eq_elim_sub_rhs_typ : mcpts.
 
-Lemma exp_eq_sub_cong_typ2 {P : PtsSig} : forall {Δ : ctx P} {Γ A σ τ s},
-    {{ Δ ⊢ A : Sort@s }} ->
+Lemma exp_eq_sub_cong_typ2 {P : PtsSig} : forall {Δ : ctx P} {Γ A σ τ},
+    {{ Δ ⊢ A }} ->
     {{ Γ ⊢s σ ≈ τ : Δ }} ->
-    {{ Γ ⊢ A[σ] ≈ A[τ] : Sort@s }}.
+    {{ Γ ⊢ A[σ] ≈ A[τ] }}.
 Proof with mautosolve 3.
-  intros.
-  gen_presups.
   mauto.
 Qed.
 
@@ -303,7 +296,7 @@ Remove Hints exp_eq_sub_cong_typ2' : mcpts.
 Lemma exp_pi_sub_lhs {P : PtsSig} : forall {Γ : ctx P} {σ Δ A B s1 s2 s3} {r : Ru P s1 s2 s3},
     {{ Γ ⊢s σ : Δ }} ->
     {{ Δ ⊢ A : Sort@s1 }} ->
-    {{ Δ, A::Sort@s1 ⊢ B : Sort@s2 }} ->
+    {{ Δ, A ⊢ B : Sort@s2 }} ->
     {{ Γ ⊢ (Π r A B)[σ] : Sort@s3 }}.
 Proof.
   intros.
@@ -316,11 +309,11 @@ Hint Resolve exp_pi_sub_lhs : mcpts.
 Lemma exp_pi_sub_rhs {P : PtsSig} : forall {Γ : ctx P} {σ Δ A B s1 s2 s3} {r : Ru P s1 s2 s3},
     {{ Γ ⊢s σ : Δ }} ->
     {{ Δ ⊢ A : Sort@s1 }} ->
-    {{ Δ, A::Sort@s1 ⊢ B : Sort@s2 }} ->
+    {{ Δ, A ⊢ B : Sort@s2 }} ->
     {{ Γ ⊢ Π r A[σ] B[q σ] : Sort@s3 }}.
 Proof.
   intros.
-  econstructor; mauto 3.
+  econstructor; mauto 4.  
 Qed.
 
 #[export]
@@ -328,53 +321,55 @@ Hint Resolve exp_pi_sub_rhs : mcpts.
 
 Lemma exp_pi_eta_rhs_body {P : PtsSig} : forall {Γ : ctx P} {A B M s1 s2 s3} {r : Ru P s1 s2 s3},
     {{ Γ ⊢ M : Π r A B }} ->
-    {{ Γ, A::Sort@s1 ⊢ M[Wk] #0 : B }}.
+    {{ Γ, A ⊢ M[Wk] #0 : B }}.
 Proof.
   intros.
   gen_presups.
-  assert ({{ Γ ⊢ A : Sort@s1 }} /\ {{ Γ, A::Sort@s1 ⊢ B : Sort@s2 }}) as [] by mauto 2.
-  assert {{ Γ, A::Sort@s1 ⊢s Wk : Γ }} by mauto 3.
-  assert {{ Γ, A::Sort@s1, A[Wk]::Sort@s1 ⊢s q Wk : Γ, A::Sort@s1 }} by mauto 3.
-  assert {{ Γ, A::Sort@s1 ⊢ M[Wk] : (Π r A B)[Wk] }} by mauto 3.
-  assert {{ Γ, A::Sort@s1 ⊢ Π r A[Wk] B[q Wk] ≈ (Π r A B)[Wk] : Sort@s3 }} by mauto 3.
-  assert {{ Γ, A::Sort@s1 ⊢ M[Wk] : Π r A[Wk] B[q Wk] }} by mauto 4.
+  assert ({{ Γ ⊢ A : Sort@s1 }} /\ {{ Γ, A ⊢ B : Sort@s2 }}) as [] by mauto 2.
+  assert {{ Γ, A ⊢s Wk : Γ }} by mauto 3.
+  assert {{ Γ, A, A[Wk] ⊢s q Wk : Γ, A }} by mauto 3.
+  assert {{ Γ, A ⊢ M[Wk] : (Π r A B)[Wk] }} by mauto 3.
+  assert {{ Γ, A ⊢ Π r A[Wk] B[q Wk] ≈ (Π r A B)[Wk] : Sort@s3 }} by mauto 3.
+  assert {{ Γ, A ⊢ M[Wk] : Π r A[Wk] B[q Wk] }} by mauto 4.
   econstructor; [econstructor; revgoals; mauto 3 | mauto 3 |]. 
-  eapply wf_typ_eq_exp.
+  (* eapply wf_typ_eq_exp. *)
   transitivity {{{ B[Wk∘Id,,#0] }}}.
   { 
     symmetry.
     eapply sub_decompose_q_typ; mauto 4.
   }
-  transitivity {{{ B[Wk,,#0] }}}; mauto.
-  eapply wf_exp_eq_conv' with (A := {{{ Sort@s2[Wk∘Id,,#0] }}}).
-  eapply wf_exp_eq_sub_cong; mauto.
-  econstructor; mauto 2.
-  eapply wf_exp_eq_conv' with (A := {{{ A[Wk] }}}); mauto.
-  eapply wf_typ_eq_sub_st with (Δ := {{{ Γ, A::Sort@s1 }}}); mauto.
-  econstructor; mauto 2.
-  do 2 (econstructor; mauto 2).
-  eapply wf_conv'; mauto.
+  transitivity {{{ B[Wk,,#0] }}}.
+  - eapply wf_typ_eq_sub_cong with (Δ := {{{ Γ, A }}}); [| mauto 3].
+    eapply wf_sub_eq_extend_cong; mauto 2.
+    eapply wf_exp_eq_conv'; mauto 3.
+    eapply wf_typ_eq_sub_cong; mauto 3.
+  - assert {{ Γ, A ⊢s Wk,,#0 ≈ Id : Γ, A }}.
+    {
+      transitivity {{{ (^(@a_weaken P)∘Id),,#0[Id] }}}; mauto.
+      eapply wf_sub_eq_extend_cong; mauto.
+    }
+    transitivity {{{ B[Id] }}}; mauto.
 Qed.
 #[export]
 Hint Resolve exp_pi_eta_rhs_body : mcpts.
 
 (** This works for both var_0 and var_S cases *)
-Lemma exp_eq_var_sub_rhs_typ_gen {P : PtsSig} : forall {Γ : ctx P} {σ Δ s A M},
+Lemma exp_eq_var_sub_rhs_typ_gen {P : PtsSig} : forall {Γ : ctx P} {σ Δ A M},
     {{ Γ ⊢s σ : Δ }} ->
-    {{ Δ ⊢ A : Sort@s }} ->
+    {{ Δ ⊢ A }} ->
     {{ Γ ⊢ M : A[σ] }} ->
-    {{ Γ ⊢ A[Wk][σ,,M] ≈ A[σ] : Sort@s }}.
+    {{ Γ ⊢ A[Wk][σ,,M] ≈ A[σ] }}.
 Proof.
   intros.
-  assert {{ Γ ⊢s σ,,M : Δ, A::Sort@s }} by mauto 3.
+  assert {{ Γ ⊢s σ,,M : Δ, A }} by mauto 3.
   transitivity {{{ A[Wk∘(σ,,M)] }}}; mauto 3.
-  eapply wf_exp_eq_conv'; mauto.
+  mauto 4.
 Qed.
 #[export]
 Hint Resolve exp_eq_var_sub_rhs_typ_gen : mcpts.
 
-Lemma exp_sub_decompose_double_q_with_id_double_extend {P : PtsSig} : forall (Γ : ctx P) A B C σ Δ M N L s1 s2,
-  {{ Γ, B::Sort@s1, C::Sort@s2 ⊢ M : A }} ->
+Lemma exp_sub_decompose_double_q_with_id_double_extend {P : PtsSig} : forall (Γ : ctx P) A B C σ Δ M N L,
+  {{ Γ, B, C ⊢ M : A }} ->
   {{ Δ ⊢s σ : Γ }} ->
   {{ Δ ⊢ N : B[σ] }} ->
   {{ Δ ⊢ L : C[σ,,N] }} ->
@@ -382,16 +377,16 @@ Lemma exp_sub_decompose_double_q_with_id_double_extend {P : PtsSig} : forall (Γ
 Proof.
   intros.
   gen_presups.
-  assert ({{ Γ ⊢ B : Sort@s1 }}) by mauto 3.
-  assert {{ Δ, B[σ]::Sort@s1 ⊢s q σ : Γ, B::Sort@s1 }} by mauto 3.
-  assert {{ Δ ⊢s Id,,N : Δ, B[σ]::Sort@s1 }} by mauto 3.
-  assert {{ Δ ⊢ L : C[q σ][Id,,N] }} by (rewrite -> @exp_eq_elim_sub_rhs_typ; mauto 3).
+  assert ({{ Γ ⊢ B }}) by mauto 3.
+  assert {{ Δ, B[σ] ⊢s q σ : Γ, B }} by mauto 3.
+  assert {{ Δ ⊢s Id,,N : Δ, B[σ] }} by mauto 3.
+  assert {{ Δ ⊢ L : C[q σ][Id,,N] }} by mauto.
   assert {{ Δ ⊢ L : C[q σ∘(Id,,N)] }} by mauto.
-  assert {{ Δ ⊢s Id,,N,,L : Δ, B[σ]::Sort@s1, C[q σ]::Sort@s2 }} by mauto 4.
-  assert {{ Δ ⊢s q σ∘(Id,,N) ≈ σ,,N : Γ, B::Sort@s1 }} by mauto 3.
-  assert {{ Δ ⊢ C[q σ][Id,,N] ≈ C[σ,,N] : Sort@s2 }} by mauto.
-  assert {{ Δ ⊢s q (q σ)∘(Id,,N,,L) ≈ (q σ∘(Id,,N)),,L : Γ, B::Sort@s1, C::Sort@s2 }} by (eapply sub_decompose_q; mauto 3).
-  assert {{ Δ ⊢s q (q σ)∘(Id,,N,,L) ≈ σ,,N,,L : Γ, B::Sort@s1, C::Sort@s2 }} by (bulky_rewrite; mauto 4).
+  assert {{ Δ ⊢s Id,,N,,L : Δ, B[σ], C[q σ] }} by mauto 4.
+  assert {{ Δ ⊢s q σ∘(Id,,N) ≈ σ,,N : Γ, B }} by mauto 3.
+  assert {{ Δ ⊢ C[q σ][Id,,N] ≈ C[σ,,N] }} by mauto.
+  assert {{ Δ ⊢s q (q σ)∘(Id,,N,,L) ≈ (q σ∘(Id,,N)),,L : Γ, B, C }} by (eapply sub_decompose_q; mauto 3).
+  assert {{ Δ ⊢s q (q σ)∘(Id,,N,,L) ≈ σ,,N,,L : Γ, B, C }} by (bulky_rewrite; mauto 4).
   assert {{ Δ ⊢ A[q (q σ)][Id,,N,,L] ≈ A[q (q σ)∘(Id,,N,,L)] }} by mauto.
   assert {{ Δ ⊢ A[q (q σ)∘(Id,,N,,L)] ≈ A[σ,,N,,L] }} by mauto.
   assert {{ Δ ⊢ M[q (q σ)][Id,,N,,L] ≈ M[q (q σ)∘(Id,,N,,L)] : A[q (q σ)∘(Id,,N,,L)] }} by mauto. 
@@ -402,37 +397,36 @@ Qed.
 #[export]
 Hint Resolve exp_sub_decompose_double_q_with_id_double_extend : mcpts.
 
-Lemma sub_eq_q_compose {P : PtsSig} : forall {Γ : ctx P} {A s σ Δ τ Δ'},
-  {{ Γ ⊢ A : Sort@s }} ->
+Lemma sub_eq_q_compose {P : PtsSig} : forall {Γ : ctx P} {A σ Δ τ Δ'},
+  {{ Γ ⊢ A }} ->
   {{ Δ ⊢s σ : Γ }} ->
   {{ Δ' ⊢s τ : Δ }} ->
-  {{ Δ', A[σ∘τ]::Sort@s ⊢s q σ∘q τ ≈ q (σ∘τ) : Γ, A::Sort@s }}.
+  {{ Δ', A[σ∘τ] ⊢s q σ∘q τ ≈ q (σ∘τ) : Γ, A }}.
 Proof.
   intros.
   assert {{ ⊢ Δ' }} by mauto 3.
-  assert {{ Δ' ⊢ A[σ∘τ] ≈ A[σ][τ] : Sort@s }} by mauto.
-  assert {{ ⊢ Δ', A[σ][τ]::Sort@s }} by mauto 4.
-  assert {{ ⊢ Δ', A[σ∘τ]::Sort@s ≈ Δ', A[σ][τ]::Sort@s }} as -> by mauto.
+  assert {{ Δ' ⊢ A[σ∘τ] ≈ A[σ][τ] }} by mauto.
+  assert {{ ⊢ Δ', A[σ][τ] }} by mauto 4.
+  assert {{ ⊢ Δ', A[σ∘τ] ≈ Δ', A[σ][τ] }} as -> by mauto.
   assert {{ ⊢ Δ }} by mauto 3.
-  assert {{ ⊢ Δ, A[σ]::Sort@s }} by mauto 3.
-  assert {{ Δ, A[σ]::Sort@s ⊢s Wk : Δ }} by mauto 3.
-  assert {{ Δ, A[σ]::Sort@s ⊢ #0 : A[σ][Wk] }} by mauto 3.
-  assert {{ Δ, A[σ]::Sort@s ⊢ #0 : A[σ∘Wk] }} by mauto 3.
+  assert {{ ⊢ Δ, A[σ] }} by mauto 3.
+  assert {{ Δ, A[σ] ⊢s Wk : Δ }} by mauto 3.
+  assert {{ Δ, A[σ] ⊢ #0 : A[σ][Wk] }} by mauto 3.
+  assert {{ Δ, A[σ] ⊢ #0 : A[σ∘Wk] }} by mauto 3.
   transitivity {{{ ((σ∘Wk)∘q τ),,#0[q τ] }}}; [econstructor; mauto 3 |].
   symmetry; econstructor; mauto 3; symmetry.
   - transitivity {{{ σ∘(Wk∘q τ) }}}; [mauto 4 |].
-    assert {{ Δ' ⊢ A[σ][τ] : Sort@s }} by mauto 3.
-    assert {{ Δ', A[σ][τ]::Sort@s ⊢s Wk : Δ' }} by mauto 3.
+    assert {{ Δ' ⊢ A[σ][τ] }} by mauto 3.
+    assert {{ Δ', A[σ][τ] ⊢s Wk : Δ' }} by mauto 3.
     transitivity {{{ σ∘(τ∘Wk) }}}; [| mauto 3].
     econstructor; mauto 3.
-  - assert {{ Δ', A[σ][τ]::Sort@s ⊢ A[(σ∘τ)∘Wk] ≈ A[σ∘(τ∘Wk)] : Sort@s }} by mauto 4.
-    assert {{ Δ', A[σ][τ]::Sort@s ⊢ A[σ∘(τ∘Wk)] ≈ A[σ][τ∘Wk] : Sort@s }} by (eapply wf_exp_eq_conv'; mauto).
-    bulky_rewrite.
-    econstructor; mauto 3.
-    assert {{ Δ', A[σ][τ]::Sort@s ⊢ A[(σ∘τ)∘Wk] ≈ A[σ][τ∘Wk] : Sort@s }} as <- by mauto 3.
-    assert {{ Δ', A[σ][τ]::Sort@s ⊢ A[(σ∘τ)∘Wk] ≈ A[σ∘τ][Wk] : Sort@s }} as -> by (eapply wf_exp_eq_conv'; mauto).
-    assert {{ Δ', A[σ][τ]::Sort@s ⊢ A[σ∘τ][Wk] ≈ A[σ][τ][Wk] : Sort@s }} as -> by (eapply wf_exp_eq_conv'; mauto 3).
-    mauto 4.
+  - assert {{ Δ', A[σ][τ] ⊢ A[(σ∘τ)∘Wk] ≈ A[σ∘(τ∘Wk)] }} by mauto 4.
+    assert {{ Δ', A[σ][τ] ⊢ A[σ∘(τ∘Wk)] ≈ A[σ][τ∘Wk] }} by mauto.
+    assert {{ Δ', A[σ][τ] ⊢ A[(σ∘τ)∘Wk] ≈ A[σ][τ∘Wk] }} by mauto 3.
+    assert {{ Δ', A[σ][τ] ⊢ A[(σ∘τ)∘Wk] ≈ A[σ∘τ][Wk] }} by mauto 4.
+    assert {{ Δ', A[σ][τ] ⊢ A[σ∘τ][Wk] ≈ A[σ][τ][Wk] }} by mauto 3.
+    eapply wf_exp_eq_conv' with (A := {{{ A[σ][τ∘Wk] }}}); mauto 3.
+    eapply wf_exp_eq_var_0_sub; mauto 4.
 Qed.
 
 #[export]
