mechanization/theories/Core/Syntactic/SystemOpt.v
@@ -53,14 +53,13 @@ Hint Resolve wf_exp_eq_conv' : mcpts.
 Remove Hints wf_exp_eq_conv : mcpts.
 
 
-Corollary wf_ctx_eq_extend' {P : PtsSig} : forall {Γ : ctx P} {Δ A A' s},
+Corollary wf_ctx_eq_extend' {P : PtsSig} : forall {Γ : ctx P} {Δ A A'},
     {{ ⊢ Γ ≈ Δ }} ->
-    {{ Γ ⊢ A ≈ A' : Sort@s }} ->
-    {{ ⊢ Γ, A::Sort@s ≈ Δ, A'::Sort@s }}.
+    {{ Γ ⊢ A ≈ A' }} ->
+    {{ ⊢ Γ, A ≈ Δ, A' }}.
 Proof.
   intros.
   gen_presups.
-  destruct_conjs.
   econstructor; mauto 2.
 Qed.
 
@@ -72,7 +71,7 @@ Remove Hints wf_ctx_eq_extend : mcpts.
 
 Corollary wf_pi {P : PtsSig} : forall {Γ : ctx P} {A B s1 s2 s3} {r : Ru P s1 s2 s3},
     {{ Γ ⊢ A : Sort@s1 }} ->
-    {{ Γ, A::Sort@s1 ⊢ B : Sort@s2 }} ->
+    {{ Γ, A ⊢ B : Sort@s2 }} ->
     {{ Γ ⊢ Π r A B : Sort@s3 }}.
 Proof.
   intros; mauto 2.
@@ -82,10 +81,11 @@ Qed.
 Hint Resolve wf_pi : mcpts.
 
 Corollary wf_fn' {P : PtsSig} : forall {Γ : ctx P} {A M B s1 s2 s3} {r : Ru P s1 s2 s3},
-    {{ Γ, A::Sort@s1 ⊢ M : B }} ->
-    {{ Γ, A::Sort@s1 ⊢ B : Sort@s2 }} ->
+    {{ Γ ⊢ A : Sort@s1 }} ->
+    {{ Γ, A ⊢ M : B }} ->
+    {{ Γ, A ⊢ B : Sort@s2 }} ->
     {{ Γ ⊢ λ r A M : Π r A B }}.
-Proof.
+Proof.  
   impl_opt_constructor.
 Qed.
 
@@ -102,10 +102,7 @@ Proof.
   intros.
   gen_presups.
   inversion_clear HAwf0.
-  assert ({{ Γ ⊢ A : Sort@s1 }} /\ {{ Γ, A::Sort@s1 ⊢ B : Sort@s2 }} /\ {{ Γ ⊢ Sort@s3 ≈ Sort@s }}) as [].
-  {
-    eapply wf_pi_inversion; mauto 2.
-  }
+  assert ({{ Γ ⊢ A : Sort@s1 }} /\ {{ Γ, A ⊢ B : Sort@s2 }} /\ {{ Γ ⊢ Sort@s3 ≈ Sort@s }}) as [] by (eapply wf_pi_inversion; mauto 2).  
   destruct_conjs.
   econstructor; mauto 2.
 Qed.
@@ -115,10 +112,9 @@ Hint Resolve wf_app' : mcpts.
 #[export]
 Remove Hints wf_app : mcpts.
 
-Lemma wf_exp_eq_typ_sub' {P : PtsSig} : forall (Γ : ctx P) σ Δ s1 s2,
-    Ax P s1 s2 ->
+Lemma wf_exp_eq_typ_sub' {P : PtsSig} : forall (Γ : ctx P) σ Δ s,
     {{ Γ ⊢s σ : Δ }} ->
-    {{ Γ ⊢ Sort@s1[σ]≈ Sort@s1 : Sort@s2 }}.
+    {{ Γ ⊢ Sort@s[σ] ≈ Sort@s}}.
 Proof.
   intros.
   econstructor; mauto 2.
@@ -133,8 +129,8 @@ Hint Rewrite -> @wf_exp_eq_typ_sub' using solve [lia | mauto 3] : mcpts.
 
 Corollary wf_exp_eq_fn_cong' {P : PtsSig} : forall {Γ : ctx P} {A A' s1 s2 s3 B M M'} {r : Ru P s1 s2 s3},
     {{ Γ ⊢ A ≈ A' : Sort@s1 }} ->
-    {{ Γ, A::Sort@s1 ⊢ M ≈ M' : B }} ->
-    {{ Γ, A::Sort@s1 ⊢ B :Sort@s2 }} ->
+    {{ Γ, A ⊢ M ≈ M' : B }} ->
+    {{ Γ, A ⊢ B :Sort@s2 }} ->
     {{ Γ ⊢ λ r A M ≈ λ r A' M' : Π r A B }}.
 Proof.
   intros.
@@ -151,8 +147,9 @@ Remove Hints wf_exp_eq_fn_cong : mcpts.
 
 Corollary wf_exp_eq_fn_sub' {P : PtsSig} : forall {Γ : ctx P} {σ Δ A M B s1 s2 s3} {r : Ru P s1 s2 s3},
     {{ Γ ⊢s σ : Δ }} ->
-    {{ Δ, A::Sort@s1 ⊢ M : B }} ->
-    {{ Δ, A::Sort@s1 ⊢ B : Sort@s2 }} ->
+    {{ Δ ⊢ A : Sort@s1 }} ->
+    {{ Δ, A ⊢ M : B }} ->
+    {{ Δ, A ⊢ B : Sort@s2 }} ->
     {{ Γ ⊢ (λ r A M)[σ] ≈ λ r A[σ] M[q σ] : (Π r A B)[σ] }}.
 Proof.
   impl_opt_constructor.
@@ -170,7 +167,7 @@ Corollary wf_exp_eq_app_cong' {P : PtsSig} : forall {Γ : ctx P} {A B M M' N N' 
 Proof.
   intros.
   gen_presups.
-  assert ({{ Γ ⊢ A : Sort@s1 }} /\ {{ Γ, A::Sort@s1 ⊢ B : Sort@s2 }}) by mauto 2.
+  assert ({{ Γ ⊢ A : Sort@s1 }} /\ {{ Γ, A ⊢ B : Sort@s2 }}) by mauto 2.
   destruct_conjs.
   econstructor; mauto 2.
 Qed.  
@@ -188,7 +185,7 @@ Corollary wf_exp_eq_app_sub' {P : PtsSig} : forall {Γ : ctx P} {σ Δ A B M N s
 Proof.
   intros.
   gen_presups.
-  assert ({{ Δ ⊢ A : Sort@s1 }} /\ {{ Δ, A::Sort@s1 ⊢ B : Sort@s2 }}) by mauto 2.
+  assert ({{ Δ ⊢ A : Sort@s1 }} /\ {{ Δ, A ⊢ B : Sort@s2 }}) by mauto 2.
   destruct_conjs.
   econstructor; mauto.
 Qed.
@@ -199,8 +196,9 @@ Hint Resolve wf_exp_eq_app_sub' : mcpts.
 Remove Hints wf_exp_eq_app_sub : mcpts.
 
 Corollary wf_exp_eq_pi_beta' {P : PtsSig} : forall {Γ : ctx P} {A B M N s1 s2 s3} {r : Ru P s1 s2 s3},
-    {{ Γ, A::Sort@s1 ⊢ M : B }} ->
-    {{ Γ, A::Sort@s1 ⊢ B : Sort@s2 }} ->
+    {{ Γ ⊢ A : Sort@s1 }} ->
+    {{ Γ, A ⊢ M : B }} ->
+    {{ Γ, A ⊢ B : Sort@s2 }} ->
     {{ Γ ⊢ N : A }} ->
     {{ Γ ⊢ (λ r A M) N ≈ M[Id,,N] : B[Id,,N] }}.
 Proof.
@@ -218,7 +216,7 @@ Corollary wf_exp_eq_pi_eta' {P : PtsSig} : forall {Γ : ctx P} {A B M s1 s2 s3} 
 Proof.
   intros.
   gen_presups.
-  assert ({{ Γ ⊢ A : Sort@s1 }} /\ {{ Γ, A::Sort@s1 ⊢ B : Sort@s2 }}) by mauto 2.
+  assert ({{ Γ ⊢ A : Sort@s1 }} /\ {{ Γ, A ⊢ B : Sort@s2 }}) by mauto 2.
   destruct_conjs.  
   econstructor; mauto 2.
 Qed.
